src/Interp.v
@@ -6,104 +6,104 @@ Require Import FreeSpec.Equiv.
 
 Local Open Scope eq_scope.
 
-Section INTERP.
-  Variable (Instruction: Type -> Type).
+CoInductive Interp
+            (I: Type -> Type)
+  : Type :=
+| interp (f: forall {A: Type}, I A -> (A * Interp I))
+  : Interp I.
 
-  CoInductive Interp: Type :=
-  | interp (f: forall {A: Type}, Instruction A -> (A * Interp))
-    : Interp.
+Arguments interp [I] (f).
 
-  Definition interpret
-             {A: Type}
-             (i: Instruction A)
-             (int: Interp)
-    : (A * Interp) :=
-    match int with interp f => f A i end.
+Definition interpret
+           {I: Type -> Type}
+           {A: Type}
+           (int: Interp I)
+           (i: I A)
+  : (A * Interp I) :=
+  match int with interp f => f A i end.
 
-  Definition evalInstruction
-             {A: Type}
-             (i: Instruction A)
-             (int: Interp)
-    : A :=
-    fst (interpret i int).
+Definition evalInstruction
+           {I: Type -> Type}
+           {A: Type}
+           (int: Interp I)
+           (i: I A)
+  : A :=
+  fst (interpret int i).
 
-  Definition execInstruction
-             {A: Type}
-             (i: Instruction A)
-             (int: Interp)
-    : Interp :=
-    snd (interpret i int).
+Definition execInstruction
+           {I: Type -> Type}
+           {A: Type}
+           (int: Interp I)
+           (i: I A)
+    : Interp I :=
+    snd (interpret int i).
 
-  CoInductive interp_eq
-              (i1: Interp)
-              (i2: Interp)
-    : Prop :=
-  | interp_is_eq (Hres: forall {A: Type}
-                              `{Eq A}
-                               (i: Instruction A),
-                     evalInstruction i i1 == evalInstruction i i2)
-                 (Hnext: forall {A: Type}
-                                (i: Instruction A),
-                     interp_eq (execInstruction i i1) (execInstruction i i2))
-    : interp_eq i1 i2.
+CoInductive interp_eq
+            {I: Type -> Type}
+            (int1: Interp I)
+            (int2: Interp I)
+  : Prop :=
+| interp_is_eq (Hres: forall {A: Type}
+                             (i: I A),
+                   evalInstruction int1 i = evalInstruction int2 i)
+               (Hnext: forall {A: Type}
+                              (i: I A),
+                   interp_eq (execInstruction int1 i) (execInstruction int2 i))
+  : interp_eq int1 int2.
 
-  Lemma interp_eq_refl
-    : forall (i: Interp), interp_eq i i.
-  Proof.
-    cofix.
-    intro i.
-    constructor.
-    + reflexivity.
-    + intros A p.
-      apply interp_eq_refl.
-  Qed.
+Lemma interp_eq_refl
+      {I: Type -> Type}
+  : forall (int: Interp I),
+    interp_eq int int.
+Proof.
+  cofix.
+  intros int.
+  constructor.
+  + reflexivity.
+  + intros A i.
+    apply interp_eq_refl.
+Qed.
 
-  Lemma interp_eq_sym
-    : forall (i i': Interp), interp_eq i i' -> interp_eq i' i.
-  Proof.
-    cofix.
-    intros int int' H1.
-    destruct H1.
-    constructor.
-    + intros A eqA i.
-      symmetry.
-      exact (Hres A eqA i).
-    + intros A i.
-      apply (interp_eq_sym (snd (interpret i int)) (snd (interpret i int')) (Hnext A i)).
-  Qed.
+Lemma interp_eq_sym
+      {I: Type -> Type}
+  : forall (int int': Interp I),
+    interp_eq int int'
+    -> interp_eq int' int.
+Proof.
+  cofix.
+  intros int int' H1.
+  destruct H1.
+  constructor.
+  + intros A i.
+    symmetry.
+    exact (Hres A i).
+  + intros A i.
+    apply (interp_eq_sym (snd (interpret int i)) (snd (interpret int' i)) (Hnext A i)).
+Qed.
 
-  Lemma interp_eq_trans
-    : forall (i i' i'': Interp),
-      interp_eq i i'
-      -> interp_eq i' i''
-      -> interp_eq i i''.
-  Proof.
-    cofix.
-    intros i i' i'' H1 H2.
-    destruct H1 as [Hres1 Hnext1].
-    destruct H2 as [Hres2 Hnext2].
-    constructor.
-    + intros A eqA p.
-      transitivity (fst (interpret p i')).
-      exact (Hres1 A eqA p).
-      exact (Hres2 A eqA p).
-    + intros A p.
-      apply (interp_eq_trans (snd (interpret p i))
-                             (snd (interpret p i'))
-                             (snd (interpret p i''))
-                             (Hnext1 A p)
-                             (Hnext2 A p)).
-  Qed.
-End INTERP.
-
-Arguments interp [_].
-Arguments interp_eq [_].
-Arguments interpret [_ _].
-Arguments evalInstruction [_ _].
-Arguments execInstruction [_ _].
-Arguments interp_eq_refl [_].
-Arguments interp_eq_sym [_].
-Arguments interp_eq_trans [_].
+Lemma interp_eq_trans
+      {I: Type -> Type}
+  : forall (int int' int'': Interp I),
+    interp_eq int int'
+    -> interp_eq int' int''
+    -> interp_eq int int''.
+Proof.
+  cofix.
+  intros int int' int'' H1 H2.
+  destruct H1 as [Hres1 Hnext1].
+  destruct H2 as [Hres2 Hnext2].
+  constructor.
+  + intros A i.
+    transitivity (fst (interpret int' i)).
+    exact (Hres1 A i).
+    exact (Hres2 A i).
+  + intros A i.
+    apply (interp_eq_trans (snd (interpret int i))
+                           (snd (interpret int' i))
+                           (snd (interpret int'' i))
+                           (Hnext1 A i)
+                           (Hnext2 A i)).
+Qed.
 
 Add Parametric Relation
     (I: Type -> Type)
@@ -116,22 +116,97 @@ Add Parametric Relation
 Instance eqInterp (I: Type -> Type): Eq (Interp I) :=
   {| equiv := @interp_eq I |}.
 
-Local Open Scope eq_scope.
+Definition run_interp_eq
+           {I: Type -> Type}
+           {A: Type}
+           (o o': (A * Interp I))
+  : Prop :=
+  fst o = fst o' /\ snd o == snd o'.
 
-Lemma _interp_int_morphism
-  : forall (I: Type -> Type)
-           (x y : Interp I)
-           (A: Type)
-           {eqA: Eq A}
-           (i: I A),
-  x == y -> (interpret i x) == (interpret i y).
+Lemma run_interp_eq_refl
+           {I: Type -> Type}
+           {A: Type}
+           (o: (A * Interp I))
+  : run_interp_eq o o.
 Proof.
-  intros I int int' A eqA i Heq.
+  constructor; reflexivity.
+Qed.
+
+Lemma run_interp_eq_sym
+           {I: Type -> Type}
+           {A: Type}
+           (o o': (A * Interp I))
+  : run_interp_eq o o'
+    -> run_interp_eq o' o.
+Proof.
+  intros [H H']; symmetry in H; symmetry in H'.
+  constructor; [exact H|exact H'].
+Qed.
+
+Lemma run_interp_eq_trans
+           {I: Type -> Type}
+           {A: Type}
+           (o o' o'': (A * Interp I))
+  : run_interp_eq o o'
+    -> run_interp_eq o' o''
+    -> run_interp_eq o o''.
+Proof.
+  intros [H H'] [G G'].
+  constructor.
+  + rewrite H; exact G.
+  + rewrite H'; exact G'.
+Qed.
+
+Add Parametric Relation
+    (I: Type -> Type)
+    (A: Type)
+  : (A * Interp I) (@run_interp_eq I A)
+    reflexivity proved by (run_interp_eq_refl)
+    symmetry proved by (run_interp_eq_sym)
+    transitivity proved by (run_interp_eq_trans)
+      as run_interp_equiv.
+
+Add Parametric Morphism
+    (I: Type -> Type)
+    (A: Type)
+  : (@fst A (Interp I))
+    with signature (run_interp_eq) ==> (@eq A)
+  as fst_program_morphism.
+Proof.
+  intros o o' [H _H].
+  exact H.
+Qed.
+
+Add Parametric Morphism
+    (I: Type -> Type)
+    (A: Type)
+  : (@snd A (Interp I))
+    with signature (run_interp_eq) ==> (interp_eq)
+  as snd_program_morphism.
+Proof.
+  intros o o' [_H H].
+  exact H.
+Qed.
+
+Instance eq_run_interp
+         {I: Type -> Type}
+         {A: Type}
+  : Eq (A * Interp I) :=
+  {| equiv := run_interp_eq |}.
+
+Add Parametric Morphism
+    (I: Type -> Type)
+    (A: Type)
+  : (interpret)
+    with signature (@interp_eq I) ==> (@eq (I A)) ==> (run_interp_eq)
+      as interp_int_morphism.
+Proof.
+  intros int int' Heq i.
   constructor.
   + destruct Heq.
-    apply (Hres A eqA i).
+    apply (Hres A i).
   + destruct Heq.
-    assert (interp_eq (snd (interpret i int)) (snd (interpret i int')))
+    assert (interp_eq (snd (interpret int i)) (snd (interpret int' i)))
       as Hin
         by (apply Hnext).
     apply Hnext.
@@ -140,46 +215,27 @@ Qed.
 Add Parametric Morphism
     (I: Type -> Type)
     (A: Type)
-    (eqA: Eq A)
-    (i: I A)
-  : (interpret i)
-    with signature (@interp_eq I) ==> (@tuple_eq A (Interp I) eqA (eqInterp I))
-      as interp_int_morphism.
-Proof.
-  intros int int' Heq.
-  constructor.
-  + destruct Heq.
-    apply (Hres A eqA i).
-  + destruct Heq.
-    assert (interp_eq (snd (interpret i int)) (snd (interpret i int'))).
-    apply (Hnext A i).
-    rewrite H.
-    reflexivity.
-Qed.
-
-Add Parametric Morphism
-    (I: Type -> Type)
-    (A: Type)
-    (eqA: Eq A)
-    (i: I A)
-  : (evalInstruction i)
-    with signature (@interp_eq I) ==> (@equiv A eqA)
+  : (evalInstruction)
+    with signature (@interp_eq I) ==> (@eq (I A)) ==> (eq)
       as eval_instr_morphism.
 Proof.
-  apply interp_int_morphism.
+  intros int int' Heq i.
+  unfold evalInstruction.
+  rewrite Heq.
+  reflexivity.
 Qed.
 
 Add Parametric Morphism
     (I: Type -> Type)
     (A: Type)
-    (eqA: Eq A)
-    (i: I A)
-  : (execInstruction i)
-    with signature (@interp_eq I) ==> (@interp_eq I)
+  : (execInstruction)
+    with signature (@interp_eq I) ==> (@eq (I A)) ==> (@interp_eq I)
       as exec_instr_morphism.
 Proof.
-  apply interp_int_morphism.
-  exact eqA.
+  intros int int' Heq i.
+  unfold execInstruction.
+  rewrite Heq.
+  reflexivity.
 Qed.
 
 (* A list of goal to check the rewrite tactic actually works *)
@@ -190,7 +246,7 @@ Goal (forall (I: Type -> Type)
              (eqA: Eq A)
              (i: I A),
          int == int'
-         -> evalInstruction i int == evalInstruction i int').
+         -> evalInstruction int i == evalInstruction int' i).
 Proof.
   intros I int int' A eqA i Heq.
   rewrite Heq.
@@ -203,7 +259,7 @@ Goal (forall (I: Type -> Type)
              (eqA: Eq A)
              (i: I A),
          int == int'
-         -> execInstruction i int == execInstruction i int').
+         -> execInstruction int i == execInstruction int' i).
 Proof.
   intros I int int' A eqA i Heq.
   rewrite Heq.
