src/Program.v
@@ -2,321 +2,387 @@ Require Import Coq.Program.Equality.
 Require Import Coq.Program.Tactics.
 Require Import Coq.Relations.Relations.
 Require Import Coq.Setoids.Setoid.
+Require Import Coq.Program.Basics.
 
-Require Import FreeSpec.Tuple.
 Require Import FreeSpec.Interp.
+Require Import FreeSpec.Equiv.
 
 Local Open Scope eq_scope.
 
-Require Import FreeSpec.Equiv.
-Section PROGRAM.
-  Variables (I: Type -> Type).
+Inductive Program
+          (I: Type -> Type)
+          (A: Type) :=
+| ret (a: A)
+  : Program I A
+| instr (i: I A)
+  : Program I A
+| bind {B: Type}
+       (p: Program I B)
+       (f: B -> Program I A)
+  : Program I A.
 
-  Inductive Program (A: Type) :=
-  | bind {B: Type}
-         (p: Program B)
-         (f: B -> Program A)
-    : Program A
-  | instr (i: I A)
-    : Program A
-  | ret (a: A)
-    : Program A.
-
-  Fixpoint runProgram
-           {A: Type}
-           (p: Program A)
-           (int: Interp I)
-    : (A * (Interp I)) :=
-    match p with
-    | ret _ a => (a, int)
-    | instr _ i => interpret i int
-    | bind _ p' f => runProgram (f (fst (runProgram p' int))) (snd (runProgram p' int))
-    end.
-
-  Definition evalProgram
-             {A: Type}
-             (p: Program A)
-             (int: Interp I)
-    : A :=
-    fst (runProgram p int).
-
-  Definition execProgram
-             {A: Type}
-             (p: Program A)
-             (int: Interp I)
-    : Interp I :=
-    snd (runProgram p int).
-
-  CoInductive program_eq
-              (i: Interp I)
-              {A: Type}
-              `{Eq A}
-              (p: Program A)
-              (p': Program A) :=
-  | program_is_eq (Hres: evalProgram p i == evalProgram p' i)
-                  (Hnext: execProgram p i == execProgram p' i)
-    : program_eq i p p'.
-
-  Lemma program_eq_refl
-        (i: Interp I)
-    : forall {A: Type}
-             `{Eq A}
-             (p: Program A),
-      program_eq i p p.
-  Proof.
-    intros A eqA p; constructor; reflexivity.
-  Qed.
-
-  Lemma program_eq_sym
-        (i: Interp I)
-    : forall {A: Type}
-             `{Eq A}
-             (p p': Program A),
-      program_eq i p p'
-      -> program_eq i p' p.
-  Proof.
-    intros A eqA p p' H1.
-    destruct H1 as [Hres Hnext].
-    constructor; symmetry; assumption.
-  Qed.
-
-  Lemma program_eq_trans
-        (i: Interp I)
-    : forall {A: Type}
-             `{Eq A}
-             (p p' p'': Program A),
-      program_eq i p p'
-      -> program_eq i p' p''
-      -> program_eq i p p''.
-  Proof.
-    intros A eqA p p' p'' [Hres1 Hnext1] [Hres2 Hnext2].
-    constructor.
-    + transitivity (evalProgram p' i); assumption.
-    + transitivity (execProgram p' i); assumption.
-  Qed.
-
-  Add Parametric Relation
-      (int: Interp I)
-      (A: Type)
-      (eqA: Eq A)
-    : (Program A) (@program_eq int A eqA)
-      reflexivity proved by (@program_eq_refl int A eqA)
-      symmetry proved by (@program_eq_sym int A eqA)
-      transitivity proved by (@program_eq_trans int A eqA)
-        as program_rel.
-
-  Definition interp_assoc
-             (int: Interp I)
-    := forall {A B C: Type}
-              `{Eq C}
-              (p: Program A)
-              (f: A -> Program B)
-              (g: B -> Program C),
-      program_eq int (bind _ (bind _ p f) g) (bind _ p (fun x => bind _ (f x) g)).
-
-  Definition interp_assoc2
-             (int: Interp I)
-    := forall {A B: Type}
-              `{Eq B}
-              (p: Program A)
-              (f: A -> Program B),
-      evalProgram (bind B p f) int
-      == evalProgram (f (evalProgram p int)) (execProgram p int).
-
-  Section CONTRACT.
-    Definition typeret
-               {A: Type}
-               (i: I A)
-    : Type := A.
-
-    Record Contract :=
-      { requirements {A: Type}
-                     (i: I A)
-        : Prop
-      ; promises {A: Type}
-                   (i: I A)
-        : typeret i -> Prop
-      }.
-
-    Variable (c: Contract).
-
-    CoInductive Enforcer
-                (int: Interp I)
-      : Prop :=
-    | enforced (Hprom: forall {A: Type}
-                              (i: I A),
-                   requirements c i
-                   -> (promises c i) (evalInstruction i int))
-               (Henf:  forall {A: Type}
-                              (i: I A),
-                   requirements c i
-                   -> Enforcer (execInstruction i int))
-      : Enforcer int.
-
-    Section PROGRAM_CONTRACT.
-      Inductive contractfull_program
-        : forall {A: Type}, Program A -> Type :=
-      | contractfull_instr {A: Type}
-                           (i: I A)
-                           (Hreq: requirements c i)
-        : contractfull_program (instr A i)
-      | contractfull_ret {A: Type}
-                         (a: A)
-        : contractfull_program (ret A a)
-      | contractfull_inv {A B: Type}
-                         (p: Program A)
-                         (f: A -> Program B)
-                         (Hcp: contractfull_program p)
-                         (Hnext: forall (int: Interp I)
-                                        (Henf: Enforcer int),
-                             contractfull_program (f (evalProgram p int)))
-        : contractfull_program (bind B p f).
-
-      Lemma contractfull_instr_enforcement
-            {A: Type}
-            (i: I A)
-        : forall (int: Interp I),
-          contractfull_program (instr A i)
-          -> Enforcer int
-          -> Enforcer (execProgram (instr A i) int).
-      Proof.
-        intros int Hc Henf.
-        destruct Henf as [Hprom Henf].
-        apply (Henf A i).
-        inversion Hc; simpl_existT; subst.
-        exact Hreq.
-      Qed.
-
-      Lemma contractfull_ret_enforcement
-            {A: Type}
-            (a: A)
-        : forall (int: Interp I),
-          contractfull_program (ret A a)
-          -> Enforcer int
-          -> Enforcer (execProgram (ret A a) int).
-      Proof.
-        intros int Hc Henf.
-        exact Henf.
-      Qed.
-
-      Lemma contractfull_program_enforcement
-            {A B: Type}
-            (p: Program A)
-        : forall (int: Interp I),
-          contractfull_program p
-          -> Enforcer int
-          -> Enforcer (execProgram p int).
-      Proof.
-        induction p.
-        + intros int Hc Henf.
-          assert (contractfull_program (f (evalProgram p int))) as Hc'.
-          ++ inversion Hc; repeat simpl_existT; subst.
-             apply (Hnext int Henf).
-          ++ inversion Hc; repeat simpl_existT; subst.
-             apply H with (int := execProgram p int) in Hc'.
-             exact Hc'.
-             apply IHp; [ exact Hcp
-                       | exact Henf
-                       ].
-        + apply contractfull_instr_enforcement.
-        + apply contractfull_ret_enforcement.
-      Qed.
-    End PROGRAM_CONTRACT.
-  End CONTRACT.
-
-  Section MAKE_INTERP.
-    Variables (State: Type).
-
-    Definition PS
-      := forall {A: Type}, State -> I A -> (A * State).
-
-    CoFixpoint mkInterp
-               (ps: PS)
-               (s: State)
-      : Interp I :=
-      interp (
-          fun (A: Type)
-              (p: I A) =>
-            (fst  (ps A s p), mkInterp ps (snd (ps A s p)))).
-
-    Lemma mkInterp_is_assoc
-          (ps: PS)
-          (s: State)
-      : interp_assoc (mkInterp ps s).
-    Proof.
-      unfold interp_assoc.
-      intros A B C p f g.
-      induction p; (constructor; [ reflexivity | apply interp_eq_refl]).
-    Qed.
-
-    Lemma mkInterp_is_assoc2
-          (ps: PS)
-          (s: State)
-      : interp_assoc2 (mkInterp ps s).
-    Proof.
-      unfold interp_assoc2.
-      intros A B p f.
-      induction p; reflexivity.
-    Qed.
-
-    Section STATEFUL_INTERP_ENFORCER.
-      Variables (step: PS)
-                (inv: State -> Prop)
-                (c: Contract).
-
-      Definition contract_preserves_inv
-        := forall {A: Type}
-                  (i: I A)
-                  (s: State),
-           inv s
-           -> requirements c i
-           -> inv (snd (step A s i)).
-
-      Definition contract_enforces_promises
-        := forall {A: Type}
-                  (i: I A)
-                  (s: State),
-          inv s
-          -> requirements c i
-          -> promises c i (fst (step A s i)).
-
-      Lemma stateful_contract_enforcement
-            (Hpres: contract_preserves_inv)
-            (Henf: contract_enforces_promises)
-        : forall (s: State), inv s -> Enforcer c (mkInterp step s).
-      Proof.
-        cofix.
-        intros s Hinv.
-        split; intros A i Hreq; cbn.
-        + apply (Henf A i s Hinv Hreq).
-        + apply (Hpres A i s) in Hinv.
-          ++ apply (stateful_contract_enforcement  (snd (step A s i)) Hinv).
-          ++ exact Hreq.
-      Qed.
-    End STATEFUL_INTERP_ENFORCER.
-  End MAKE_INTERP.
-End PROGRAM.
-
-Arguments bind [I A B] (p f).
-Arguments instr [I A] (i).
 Arguments ret [I A] (a).
+Arguments instr [I A] (i).
+Arguments bind [I A B] (p f).
 
-Arguments mkInterp [I State] (ps s).
+Fixpoint runProgram
+         {I: Type -> Type}
+         {A: Type}
+         (int: Interp I)
+         (p: Program I A)
+  : (A * Interp I) :=
+  match p with
+  | ret a => (a, int)
+  | instr i => interpret int i
+  | bind p' f => runProgram (snd (runProgram int p')) (f (fst (runProgram int p')))
+  end.
 
-Arguments runProgram [I A] (p int).
-Arguments execProgram [I A] (p int).
-Arguments evalProgram [I A] (p int).
+Definition evalProgram
+           {I: Type -> Type}
+           {A: Type}
+           (int: Interp I)
+           (p: Program I A)
+  : A :=
+  fst (runProgram int p).
 
-Arguments typeret [I A] (i).
-Arguments Enforcer [I] (c int).
+Definition execProgram
+           {I: Type -> Type}
+           {A: Type}
+           (int: Interp I)
+           (p: Program I A)
+  : Interp I :=
+  snd (runProgram int p).
 
-Arguments stateful_contract_enforcement [I State] (step inv c Hpres Henf s).
-Arguments contract_enforces_promises [I State] (step inv c).
-Arguments contract_preserves_inv [I State] (step inv c).
+CoInductive program_eq
+            {I: Type -> Type}
+            {A: Type}
+            (p: Program I A)
+            (p': Program I A) :=
+| program_is_eq (Hres: forall (int: Interp I),
+                    evalProgram int p = evalProgram int p')
+                (Hnext: forall (int: Interp I),
+                    execProgram int p == execProgram int p')
+  : program_eq p p'.
 
-Arguments contractfull_program [I] c [A].
+Lemma program_eq_refl
+      {I: Type -> Type}
+      {A: Type}
+      (p: Program I A)
+  : program_eq p p.
+Proof.
+  constructor; reflexivity.
+Qed.
 
-Notation "int <· p" := (fst (runProgram int p)) (at level 50) : prog_scope.
+Lemma program_eq_sym
+      {I: Type -> Type}
+      {A: Type}
+      (p p': Program I A)
+  : program_eq p p'
+    -> program_eq p' p.
+Proof.
+  intro H1.
+  destruct H1 as [Hres Hnext].
+  constructor.
+  + intro int.
+    rewrite Hres.
+    reflexivity.
+  + intro int.
+    rewrite Hnext.
+    reflexivity.
+Qed.
+
+Lemma program_eq_trans
+      {I: Type -> Type}
+      {A: Type}
+      (p p' p'': Program I A)
+  : program_eq p p'
+    -> program_eq p' p''
+    -> program_eq p p''.
+Proof.
+  intros [Hres1 Hnext1] [Hres2 Hnext2].
+  constructor; intro int.
+  + transitivity (evalProgram int p').
+    ++ apply Hres1.
+    ++ apply Hres2.
+  + transitivity (execProgram int p').
+    ++ apply Hnext1.
+    ++ apply Hnext2.
+Qed.
+
+Add Parametric Relation
+    (I: Type -> Type)
+    (A: Type)
+  : (Program I A) (program_eq)
+    reflexivity proved by (program_eq_refl)
+    symmetry proved by (program_eq_sym)
+    transitivity proved by (program_eq_trans)
+      as program_equiv.
+
+Lemma interp_assoc
+      {I: Type -> Type}
+      {A B C: Type}
+      (p: Program I A)
+      (f: A -> Program I B)
+      (g: B -> Program I C)
+  : program_eq (bind (bind p f) g) (bind p (fun x => bind (f x) g)).
+Proof.
+  constructor.
+  + reflexivity.
+  + reflexivity.
+Qed.
+
+Lemma interp_assoc2
+           {I: Type -> Type}
+           {A B: Type}
+           (int: Interp I)
+           (p: Program I A)
+           (f: A -> Program I B)
+  : runProgram int (bind p f)
+    == runProgram (execProgram int p) (f (evalProgram int p)).
+Proof.
+  reflexivity.
+Qed.
+
+Add Parametric Morphism
+    (I: Type -> Type)
+    (A: Type)
+  : (runProgram)
+    with signature eq ==> (program_eq) ==> (@run_interp_eq I A)
+  as run_program_morphism.
+Proof.
+  intros y p p' Heq.
+  constructor.
+  destruct Heq.
+  + apply Hres.
+  + apply Heq.
+Qed.
+
+Add Parametric Morphism
+    (I: Type -> Type)
+    (A: Type)
+  : (evalProgram)
+    with signature eq ==> (@program_eq I A) ==> (eq)
+  as eval_program_morphism.
+Proof.
+  intros y p p' Heq.
+  unfold evalProgram.
+  rewrite Heq.
+  reflexivity.
+Qed.
+
+Add Parametric Morphism
+    (I: Type -> Type)
+    (A: Type)
+  : (execProgram)
+    with signature eq ==> (@program_eq I A) ==> (@interp_eq I)
+  as exec_program_morphism.
+Proof.
+  intros y p p' Heq.
+  unfold execProgram.
+  rewrite Heq.
+  reflexivity.
+Qed.
+
+Definition typeret
+           {I: Type -> Type}
+           {A: Type}
+           (i: I A)
+  : Type := A.
+
+Record Contract
+       (I: Type -> Type) :=
+  { requirements {A: Type}
+                 (i: I A)
+    : Prop
+  ; promises {A: Type}
+             (i: I A)
+    : typeret i -> Prop
+  }.
+
+Arguments requirements [I] (c) [A] (i).
+Arguments promises [I] (c) [A] (i _).
+
+CoInductive Enforcer
+            {I: Type -> Type}
+            (c: Contract I)
+            (int: Interp I)
+  : Prop :=
+| enforced (Hprom: forall {A: Type}
+                          (i: I A),
+               requirements c i
+               -> (promises c i) (evalInstruction int i))
+           (Henf:  forall {A: Type}
+                          (i: I A),
+               requirements c i
+               -> Enforcer c (execInstruction int i))
+  : Enforcer c int.
+
+Add Parametric Morphism
+    (I: Type -> Type)
+    (c: Contract I)
+  : (Enforcer c)
+    with signature (@interp_eq I) ==> (impl)
+      as enforcer_morphism.
+Proof.
+  cofix.
+  intros int int' Heq He.
+  constructor.
+  + intros A i Hreq.
+    rewrite <- Heq.
+    destruct He.
+    apply Hprom.
+    exact Hreq.
+  + intros A i Hreq.
+    destruct He.
+    apply Henf in Hreq.
+    apply (enforcer_morphism_Proper (execInstruction int i) (execInstruction int' i)) in Hreq.
+    ++ exact Hreq.
+    ++ destruct Heq.
+       apply Hnext.
+Qed.
+
+Inductive contractfull_program
+          {I: Type -> Type}
+          (c: Contract I)
+  : forall {A: Type}, Program I A -> Type :=
+| contractfull_instr {A: Type}
+                     (i: I A)
+                     (Hreq: requirements c i)
+  : contractfull_program c (instr i)
+| contractfull_ret {A: Type}
+                   (a: A)
+  : contractfull_program c (ret a)
+| contractfull_inv {A B: Type}
+                   (p: Program I A)
+                   (f: A -> Program I B)
+                   (Hcp: contractfull_program c p)
+                   (Hnext: forall (int: Interp I)
+                                  (Henf: Enforcer c int),
+                       contractfull_program c (f (evalProgram int p)))
+  : contractfull_program c (bind p f).
+
+Lemma contractfull_instr_enforcement
+      {I: Type -> Type}
+      {A: Type}
+      {c: Contract I}
+      {i: I A}
+      {int: Interp I}
+      (Hc: contractfull_program c (instr i))
+      (Henf: Enforcer c int)
+  : Enforcer c (execProgram int (instr i)).
+Proof.
+  destruct Henf as [Hprom Henf].
+  apply (Henf A i).
+  inversion Hc; simpl_existT; subst.
+  exact Hreq.
+Qed.
+
+Lemma contractfull_ret_enforcement
+      {I: Type -> Type}
+      {A: Type}
+      {c: Contract I}
+      (a: A)
+      {int: Interp I}
+      (He: Enforcer c int)
+  : Enforcer c (execProgram int (ret a)).
+Proof.
+  exact He.
+Qed.
+
+Lemma contractfull_program_enforcement
+      {I: Type -> Type}
+      {A B: Type}
+      (c: Contract I)
+      (p: Program I A)
+  : forall (int: Interp I)
+           (Hc: contractfull_program c p)
+           (He: Enforcer c int),
+    Enforcer c (execProgram int p).
+Proof.
+  induction p.
+  + intros int Hc He.
+    apply (contractfull_ret_enforcement a He).
+  + intros int Hc He.
+    apply (contractfull_instr_enforcement Hc He).
+  + intros int Hc He.
+    assert (contractfull_program c (f (evalProgram int p))) as Hc'.
+    ++ inversion Hc; repeat simpl_existT; subst.
+       apply (Hnext int He).
+    ++ inversion Hc; repeat simpl_existT; subst.
+       apply H with (int:=execProgram int p) in Hc'.
+       exact Hc'.
+       apply IHp.
+       +++ exact Hcp.
+       +++ exact He.
+Qed.
+
+Definition PS
+           {I: Type -> Type}
+           (State: Type)
+  := forall {A: Type}, State -> I A -> (A * State).
+
+CoFixpoint mkInterp
+           {I: Type -> Type}
+           {State: Type}
+           (ps: PS State)
+           (s: State)
+  : Interp I :=
+  interp (
+      fun (A: Type)
+          (p: I A) =>
+        (fst  (ps A s p), mkInterp ps (snd (ps A s p)))).
+
+Definition contract_preserves_inv
+            {I: Type -> Type}
+            {State: Type}
+            (c: Contract I)
+            (inv: State -> Prop)
+            (step: PS State)
+  := forall {A: Type}
+            (i: I A)
+            (s: State),
+     inv s
+     -> requirements c i
+     -> inv (snd (step A s i)).
+
+Definition contract_enforces_promises
+            {I: Type -> Type}
+            {State: Type}
+            (c: Contract I)
+            (inv: State -> Prop)
+            (step: PS State)
+  := forall {A: Type}
+            (i: I A)
+            (s: State),
+    inv s
+    -> requirements c i
+    -> promises c i (fst (step A s i)).
+
+Lemma stateful_contract_enforcement
+      {I: Type -> Type}
+      {State: Type}
+      (c: Contract I)
+      (inv: State -> Prop)
+      (step: PS State)
+      (Hpres: contract_preserves_inv c inv step)
+      (Henf: contract_enforces_promises c inv step)
+  : forall {A: Type}
+           (i: I A)
+           (s: State)
+  , inv s
+    -> Enforcer c (mkInterp step s).
+Proof.
+  cofix.
+  intros A i s Hinv.
+  constructor.
+  + intros B i' Hreq.
+    apply (Henf B i' s Hinv Hreq).
+  + intros B i' Hreq.
+    apply (Hpres B i' s) in Hinv.
+    ++ apply (stateful_contract_enforcement B i' (snd (step B s i')) Hinv).
+    ++ exact Hreq.
+Qed.
+
 Notation "p >>= f" := (bind p f) (at level 50) : prog_scope.
 Notation "a <- p ; q" :=
   (bind p (fun a => q)) (at level 60, right associativity, p at next level)
