src/TemporalLogic.v
@@ -1,671 +1,754 @@
+Require Import Coq.Program.Equality.
 Require Import Coq.Bool.Sumbool.
 Require Import Coq.Logic.Classical.
+Require Import Coq.Setoids.Setoid.
+
 Require Import FreeSpec.Utils.
 Require Import FreeSpec.Interp.
 Require Import FreeSpec.Program.
+Require Import FreeSpec.Equiv.
 
-Section TEMPORAL_LOGIC.
-  Variables (A: Type)
-            (I: Type -> Type).
+Record Instant
+       (A: Type) :=
+  { prop: A -> Prop
+  ; prop_dec: forall (a: A), {prop a}+{~prop a}
+  }.
 
-  Record Instant :=
-    { prop: A -> Prop
-    ; prop_dec: forall (a: A), {prop a}+{~prop a}
-    }.
-
-  Notation "p ? a" := (prop_dec p a) (at level 51).
-  Notation "p .? a" := (prop p a) (at level 51).
-
-  Definition prop_eq
-             (p p': Instant)
-    : Prop :=
-    forall (a: A), p .? a <-> p' .? a.
-
-  Lemma prop_eq_refl
-        (p: Instant)
-    : prop_eq p p.
-  Proof.
-    intro a; split; intro Hp; exact Hp.
-  Qed.
-
-  Lemma prop_eq_sym
-        (p p': Instant)
-    : prop_eq p p'
-      -> prop_eq p' p.
-  Proof.
-    intros Hp a.
-    split; intro Hp'; destruct (Hp a) as [H1 H2].
-    + apply (H2 Hp').
-    + apply (H1 Hp').
-  Qed.
-
-  Lemma prop_eq_trans
-        (p p' p'': Instant)
-    : prop_eq p p'
-      -> prop_eq p' p''
-      -> prop_eq p p''.
-  Proof.
-    intros H1 H2 a.
-    destruct (H1 a) as [H1_1 H1_2].
-    destruct (H2 a) as [H2_1 H2_2].
-    split; intro H.
-    + apply (H2_1 (H1_1 H)).
-    + apply (H1_2 (H2_2 H)).
-  Qed.
-
-  Add Parametric Relation: (Instant) (prop_eq)
-      reflexivity proved by (prop_eq_refl)
-      symmetry proved by (prop_eq_sym)
-      transitivity proved by (prop_eq_trans)
-        as prop_eq_rel.
-
-  Inductive TL: Type :=
-  | true
-    : TL
-  | false
-    : TL
-  | globally (prop: Instant)
-    : TL
-  | eventually (prop: Instant)
-    : TL
-  | next (tl: TL)
-    : TL
-  | switch (tl1: TL)
-           (prop: Instant)
-           (tl2: TL)
-    : TL.
-
-  Fixpoint halt_satisfies
-             (tl: TL)
-    : Prop :=
-    match tl with
-    | eventually _ => False
-    | next _ => False
-    | switch before _ _ => halt_satisfies before
-    | _ => True
-    end.
-
-  Fixpoint halt_satisfies_dec
-          (tl: TL)
-    : {halt_satisfies tl}+{~halt_satisfies tl}.
-    refine (
-        match tl with
-        | eventually _ => false_dec
-        | next _ => false_dec
-        | switch before _ _ => decide_dec (halt_satisfies_dec before)
-        | _ => true_dec
-        end);
-      cbn;
-      firstorder.
-    Defined.
-
-  Inductive TL_step
-    : TL -> TL -> Prop :=
-  | true_stays_true: TL_step true true
-  | false_stays_false: TL_step false false
-  | globally_stays_globally
-      (prop: Instant)
-    : TL_step (globally prop) (globally prop)
-  | globally_can_fail
-      (prop: Instant)
-    : TL_step (globally prop) false
-  | eventually_stays_eventually
-      (prop: Instant)
-    : TL_step (eventually prop) (eventually prop)
-  | eventually_can_succeed
-      (prop: Instant)
-    : TL_step (eventually prop) true
-  | next_steps_unwrap
-      (tl: TL)
-    : TL_step (next tl) tl
-  | switch_steps_before
-      (tl1 tl2 tl3: TL)
-      (prop: Instant)
-      (Hderive: TL_step tl1 tl2)
-    : TL_step (switch tl1 prop tl3) (switch tl2 prop tl3)
-  | switch_step_after_small
-      (tl1 tl2: TL)
-      (prop: Instant)
-    : TL_step (switch tl1 prop tl2) tl2
-  | switch_can_fail
-      (tl1 tl2: TL)
-      (prop: Instant)
-    : TL_step (switch tl1 prop tl2) false.
-
-  Fixpoint instruction_satisfies
-           (a: A)
-           (tl: TL)
-    : Prop :=
-    match tl with
-    | true => True
-    | false => False
-    | globally prop => prop.? a
-    | eventually tl => True
-    | next _
-      => True
-    | switch before prop after
-      => (prop.? a -> instruction_satisfies a after
-                      /\ halt_satisfies before)
-         /\ (~prop.? a -> instruction_satisfies a before)
-    end.
-
-  Fixpoint instruction_satisfies_dec
-          (a: A)
-          (tl: TL)
-    : {instruction_satisfies a tl}+{~instruction_satisfies a tl}.
-    refine (
-        match tl with
-        | true
-          => true_dec
-        | false
-          => false_dec
-        | globally prop
-          => decide_dec (prop? a)
-        | eventually prop
-          => true_dec
-        | next _
-          => true_dec
-        | switch before p after
-          => if p? a
-             then decide_dec (sumbool_and _ _ _ _
-                                          (instruction_satisfies_dec a after)
-                                          (halt_satisfies_dec before))
-             else decide_dec (instruction_satisfies_dec a before)
-        end
-      ); cbn; trivial.
-    + intro False; destruct False.
-    + split.
-      ++ intro _H; exact a0.
-      ++ intro False; apply False in p0; destruct p0.
-    + intro False.
-      destruct False as [False _H].
-      apply False in p0.
-      apply or_not_and in o.
-      apply o in p0.
-      destruct p0.
-    + split.
-      ++ intro False; apply n in False; destruct False.
-      ++ intro _H; exact i.
-    + intro False.
-      destruct False as [_H False].
-      apply False in n.
-      apply n0 in n.
-      destruct n.
-  Defined.
-
-  Fixpoint tl_step
-           (a: A)
-           (tl: TL)
-    : TL :=
-    if instruction_satisfies_dec a tl
-    then match tl with
-         | next tl
-           => tl
-         | switch before p after
-           => if p? a
-              then after
-              else switch (tl_step a before) p after
-         | eventually p
-           => if p ? a
-              then true
-              else eventually p
-         | x
-           => x
-         end
-    else false.
-
-  Lemma TL_step_is_tl_step
-    : forall (a: A)
-             (tl: TL),
-      TL_step tl (tl_step a tl).
-  Proof.
-    induction tl.
-    + constructor.
-    + constructor.
-    + cbn; destruct (prop0 ? a); constructor.
-    + cbn; destruct (prop0 ? a); constructor.
-    + cbn; constructor.
-    + cbn.
-      destruct (prop0 ? a).
-      ++ destruct (instruction_satisfies_dec a tl2);
-           destruct (halt_satisfies_dec tl1);
-           cbn.
-         +++ constructor.
-         +++ constructor.
-         +++ constructor.
-         +++ constructor.
-      ++ destruct (instruction_satisfies_dec a tl1).
-         +++ constructor.
-             exact IHtl1.
-         +++ constructor.
-  Qed.
-
-End TEMPORAL_LOGIC.
-
-Arguments true [_].
-Arguments false [_].
-Arguments next [_].
-Arguments globally [_].
-Arguments eventually [_].
-Arguments switch [_].
-
-Arguments TL_step [_].
-Arguments tl_step [_].
-
-Arguments prop_dec [_].
-Arguments prop [_].
+Arguments prop [A] (_ _).
+Arguments prop_dec [A] (_ _).
 
 Notation "p ? a" := (prop_dec p a) (at level 51): instant_scope.
 Notation "p .? a" := (prop p a) (at level 51): instant_scope.
 
-Section RUN_TL.
-  Variable (I: Type -> Type).
+Local Open Scope instant_scope.
+Local Open Scope eq_scope.
 
-  Local Open Scope instant_scope.
+Inductive TL
+          (A: Type)
+  : Type :=
+| true
+  : TL A
+| false
+  : TL A
+| globally (prop: Instant A)
+  : TL A
+| eventually (prop: Instant A)
+  : TL A
+| next (tl: TL A)
+  : TL A
+| switch (tl1: TL A)
+         (prop: Instant A)
+         (tl2: TL A)
+  : TL A.
 
-  Inductive ISet: Type :=
+Arguments true [_].
+Arguments false [_].
+Arguments globally [_] (_).
+Arguments eventually [_] (_).
+Arguments next [_] (_).
+Arguments switch [_] (_ _ _).
+
+Fixpoint halt_satisfies
+         {A: Type}
+         (tl: TL A)
+  : Prop :=
+  match tl with
+  | eventually _ => False
+  | next _ => False
+  | switch before _ _ => halt_satisfies before
+  | _ => True
+  end.
+
+Fixpoint halt_satisfies_dec
+         {A: Type}
+         (tl: TL A)
+  : {halt_satisfies tl}+{~halt_satisfies tl}.
+  refine (
+      match tl with
+      | eventually _ => false_dec
+      | next _ => false_dec
+      | switch before _ _ => decide_dec (halt_satisfies_dec A before)
+      | _ => true_dec
+      end);
+    cbn;
+    firstorder.
+Defined.
+
+Inductive TL_step
+          {A: Type}
+  : TL A -> TL A -> Prop :=
+| true_stays_true: TL_step true true
+| false_stays_false: TL_step false false
+| globally_stays_globally
+    (prop: Instant A)
+  : TL_step (globally prop) (globally prop)
+| globally_can_fail
+    (prop: Instant A)
+  : TL_step (globally prop) false
+| eventually_stays_eventually
+    (prop: Instant A)
+  : TL_step (eventually prop) (eventually prop)
+| eventually_can_succeed
+    (prop: Instant A)
+  : TL_step (eventually prop) true
+| next_steps_unwrap
+    (tl: TL A)
+  : TL_step (next tl) tl
+| switch_steps_before
+    (tl1 tl2 tl3: TL A)
+    (prop: Instant A)
+    (Hderive: TL_step tl1 tl2)
+  : TL_step (switch tl1 prop tl3) (switch tl2 prop tl3)
+| switch_step_after_small
+    (tl1 tl2: TL A)
+    (prop: Instant A)
+  : TL_step (switch tl1 prop tl2) tl2
+| switch_can_fail
+    (tl1 tl2: TL A)
+    (prop: Instant A)
+  : TL_step (switch tl1 prop tl2) false.
+
+Arguments true_stays_true [_].
+Arguments false_stays_false [_].
+Arguments globally_stays_globally [_] (_).
+Arguments globally_can_fail [_] (_).
+Arguments eventually_stays_eventually [_] (_).
+Arguments eventually_can_succeed [_] (_).
+Arguments next_steps_unwrap [_] (_).
+Arguments switch_steps_before [_] (_ _ _ _ _).
+Arguments switch_step_after_small [_] (_ _ _).
+Arguments switch_can_fail [_] (_ _ _).
+
+Fixpoint instruction_satisfies
+         {A: Type}
+         (a: A)
+         (tl: TL A)
+  : Prop :=
+  match tl with
+  | true => True
+  | false => False
+  | globally prop => prop.? a
+  | eventually tl => True
+  | next _
+    => True
+  | switch before prop after
+    => (prop.? a -> instruction_satisfies a after
+                    /\ halt_satisfies before)
+       /\ (~prop.? a -> instruction_satisfies a before)
+  end.
+
+Fixpoint instruction_satisfies_dec
+         {A: Type}
+         (a: A)
+         (tl: TL A)
+  : {instruction_satisfies a tl}+{~instruction_satisfies a tl}.
+  refine (
+      match tl with
+      | true
+        => true_dec
+      | false
+        => false_dec
+      | globally prop
+        => decide_dec (prop? a)
+      | eventually prop
+        => true_dec
+      | next _
+        => true_dec
+      | switch before p after
+        => if p? a
+           then decide_dec (sumbool_and _ _ _ _
+                                        (instruction_satisfies_dec A a after)
+                                        (halt_satisfies_dec before))
+           else decide_dec (instruction_satisfies_dec A a before)
+      end
+    ); cbn; trivial.
+  + intro False; destruct False.
+  + split.
+    ++ intro _H; exact a0.
+    ++ intro False; apply False in p0; destruct p0.
+  + intro False.
+    destruct False as [False _H].
+    apply False in p0.
+    apply or_not_and in o.
+    apply o in p0.
+    destruct p0.
+  + split.
+    ++ intro False; apply n in False; destruct False.
+    ++ intro _H; exact i.
+  + intro False.
+    destruct False as [_H False].
+    apply False in n.
+    apply n0 in n.
+    destruct n.
+Defined.
+
+Fixpoint tl_step
+         {A: Type}
+         (a: A)
+         (tl: TL A)
+  : TL A :=
+  if instruction_satisfies_dec a tl
+  then match tl with
+       | next tl
+         => tl
+       | switch before p after
+         => if p? a
+            then after
+            else switch (tl_step a before) p after
+       | eventually p
+         => if p ? a
+            then true
+            else eventually p
+       | x
+         => x
+       end
+  else false.
+
+Lemma TL_step_is_tl_step
+      {A: Type}
+      (a: A)
+      (tl: TL A)
+  : TL_step tl (tl_step a tl).
+Proof.
+  induction tl.
+  + constructor.
+  + constructor.
+  + cbn; destruct (prop0 ? a); constructor.
+  + cbn; destruct (prop0 ? a); constructor.
+  + cbn; constructor.
+  + cbn.
+    destruct (prop0 ? a).
+    ++ destruct (instruction_satisfies_dec a tl2);
+         destruct (halt_satisfies_dec tl1);
+         cbn.
+       +++ constructor.
+       +++ constructor.
+       +++ constructor.
+       +++ constructor.
+    ++ destruct (instruction_satisfies_dec a tl1).
+       +++ constructor.
+           exact IHtl1.
+       +++ constructor.
+Qed.
+
+Inductive ISet
+          (I: Type -> Type)
+  : Type :=
   | instruction {A: Type}
                 (i: I A)
-    : ISet.
+    : ISet I.
 
-  Fixpoint runTL
+Arguments instruction [_ _].
+
+Fixpoint runTL
+         {I: Type -> Type}
+         {A: Type}
+         (int: Interp I)
+         (p: Program I A)
+         (tl: TL (ISet I))
+  : (A * (Interp I) * TL (ISet I)) :=
+  match p with
+  | ret a => (a, int, tl)
+  | instr i => (evalInstruction int i,
+                execInstruction int i,
+                tl_step (instruction i) tl)
+  | bind p' f => runTL (snd (fst (runTL int p' tl)))
+                       (f (fst (fst (runTL int p' tl))))
+                       (snd (runTL int p' tl))
+  end.
+
+Definition evalTL
+           {I: Type -> Type}
            {A: Type}
            (int: Interp I)
            (p: Program I A)
-           (tl: TL (ISet))
-    : (A * (Interp I) * TL (ISet)) :=
-    match p with
-    | ret a => (a, int, tl)
-    | instr i => (evalInstruction i int,
-                    execInstruction i int,
-                    tl_step (instruction i) tl)
-    | bind p' f => runTL (snd (fst (runTL int p' tl)))
-                         (f (fst (fst (runTL int p' tl))))
-                         (snd (runTL int p' tl))
-    end.
+           (tl: TL (ISet I))
+  : A :=
+  fst (fst (runTL int p tl)).
 
-  Definition evalTL
-             {A: Type}
-             (int: Interp I)
-             (p: Program I A)
-             (tl: TL (ISet))
-    : A :=
-    fst (fst (runTL int p tl)).
+Definition execTL
+           {I: Type -> Type}
+           {A: Type}
+           (int: Interp I)
+           (p: Program I A)
+           (tl: TL (ISet I))
+  : Interp I :=
+  snd (fst (runTL int p tl)).
 
-  Definition execTL
-             {A: Type}
-             (int: Interp I)
-             (p: Program I A)
-             (tl: TL (ISet))
-    : Interp I :=
-    snd (fst (runTL int p tl)).
+Definition deriveTL
+           {I: Type -> Type}
+           {A: Type}
+           (int: Interp I)
+           (p: Program I A)
+           (tl: TL (ISet I))
+  : TL (ISet I) :=
+  snd (runTL int p tl).
 
-  Definition deriveTL
-             {A: Type}
-             (int: Interp I)
-             (p: Program I A)
-             (tl: TL (ISet))
-    : TL (ISet) :=
-    snd (runTL int p tl).
+Lemma run_tl_run_program_same
+      {I: Type -> Type}
+      {A: Type}
+  : forall (p: Program I A)
+           (tl: TL (ISet I))
+           (int: Interp I),
+    fst (runTL int p tl) = runProgram int p.
+Proof.
+  induction p; intros tl int; cbn.
+  + reflexivity.
+  + apply injective_projections; reflexivity.
+  + rewrite H; rewrite IHp; reflexivity.
+Qed.
 
-  Inductive TL_run
-            {A: Type}
-    : TL A -> TL A -> Prop :=
-  | tl_run_refl
-      (tl: TL A)
-    : TL_run tl tl
-  | tl_run_small_step
-      (from to: TL A)
-      (Hstep: TL_step from to)
-    : TL_run from to
-  | tl_run_big_step
-      (from tl to: TL A)
-      (Hstep: TL_step from tl)
-      (Hrun: TL_run tl to)
-    : TL_run from to.
+Lemma exec_tl_exec_program_same
+      {I: Type -> Type}
+      {A: Type}
+  : forall (p: Program I A)
+           (tl: TL (ISet I))
+           (int: Interp I),
+    execTL int p tl = execProgram int p.
+Proof.
+  intros p tl int.
+  unfold execTL, execProgram.
+  rewrite run_tl_run_program_same.
+  reflexivity.
+Qed.
 
-  Lemma tl_step_run_trans
-        {A: Type}
-        (tl tl' tl'': TL A)
-    : TL_step tl tl'
-      -> TL_step tl' tl''
-      -> TL_run tl tl''.
-  Proof.
-    intros H1 H2.
-    apply (tl_run_big_step tl tl' tl'').
-    + exact H1.
-    + apply (tl_run_small_step tl' tl'' H2).
-  Qed.
+Lemma eval_tl_eval_program_same
+      {I: Type -> Type}
+      {A: Type}
+  : forall (p: Program I A)
+           (tl: TL (ISet I))
+           (int: Interp I),
+    evalTL int p tl = evalProgram int p.
+Proof.
+  intros p tl int.
+  unfold evalTL, execProgram.
+  rewrite run_tl_run_program_same.
+  reflexivity.
+Qed.
 
-  Lemma tl_run_step_run
-        {A: Type}
-        (tl tl' tl'': TL A)
-    : TL_run tl tl'
-      -> TL_step tl' tl''
-      -> TL_run tl tl''.
-  Proof.
-    intros H1 H2.
-    induction H1.
-    ++ constructor.
-       exact H2.
-    ++ apply (tl_step_run_trans from to tl'' Hstep H2).
-    ++ apply IHTL_run in H2.
-       apply (tl_run_big_step from tl tl'' Hstep H2).
-  Qed.
+Add Parametric Morphism
+    (I: Type -> Type)
+    (A: Type)
+  : (evalTL)
+    with signature (eq) ==> (@program_eq I A) ==> (eq) ==> (eq)
+      as eval_tl_morphism.
+Proof.
+  intros int p p' Heq tl.
+  unfold evalTL.
+  rewrite run_tl_run_program_same.
+  rewrite run_tl_run_program_same.
+  rewrite Heq.
+  reflexivity.
+Qed.
 
-  Lemma tl_run_trans
-        {A: Type}
-        (tl tl' tl'': TL A)
-    : TL_run tl tl'
-      -> TL_run tl' tl''
-      -> TL_run tl tl''.
-  Proof.
-    intros H1 H2.
-    induction H1.
-    + exact H2.
-    + apply (tl_run_big_step from to tl'' Hstep H2).
-    + apply IHTL_run in H2.
-      apply (tl_run_big_step from tl tl'' Hstep H2).
-  Qed.
+Add Parametric Morphism
+    (I: Type -> Type)
+    (A: Type)
+  : (execTL)
+    with signature (eq) ==> (@program_eq I A) ==> (eq) ==> (@interp_eq I)
+      as exec_tl_morphism.
+Proof.
+  intros int p p' Heq tl.
+  unfold execTL.
+  rewrite run_tl_run_program_same.
+  rewrite run_tl_run_program_same.
+  rewrite Heq.
+  reflexivity.
+Qed.
 
-  Lemma next_derives_big
+Lemma run_tl_bind_ret
+      {I: Type -> Type}
+      {A B: Type}
+      (int: Interp I)
+      (a: A)
+      (f: A -> Program I B)
+      (tl: TL (ISet I))
+  : runTL int (bind (ret a) f) tl = runTL int (f a) tl.
+Proof.
+  reflexivity.
+Qed.
+
+Lemma exec_tl_bind_ret
+      {I: Type -> Type}
+      {A B: Type}
+      (int: Interp I)
+      (a: A)
+      (f: A -> Program I B)
+      (tl: TL (ISet I))
+  : execTL int (bind (ret a) f) tl = execTL int (f a) tl.
+Proof.
+  reflexivity.
+Qed.
+
+Lemma derive_tl_bind_ret
+      {I: Type -> Type}
+      {A B: Type}
+      (int: Interp I)
+      (a: A)
+      (f: A -> Program I B)
+      (tl: TL (ISet I))
+  : deriveTL int (bind (ret a) f) tl = deriveTL int (f a) tl.
+Proof.
+  reflexivity.
+Qed.
+
+Inductive TL_run
+          {A: Type}
+  : TL A -> TL A -> Prop :=
+| tl_run_refl
+    (tl: TL A)
+  : TL_run tl tl
+| tl_run_small_step
+    (from to: TL A)
+    (Hstep: TL_step from to)
+  : TL_run from to
+| tl_run_big_step
+    (from tl to: TL A)
+    (Hstep: TL_step from tl)
+    (Hrun: TL_run tl to)
+  : TL_run from to.
+
+Lemma tl_step_run_trans
+      {A: Type}
+      (tl tl' tl'': TL A)
+  : TL_step tl tl'
+    -> TL_step tl' tl''
+    -> TL_run tl tl''.
+Proof.
+  intros H1 H2.
+  apply (tl_run_big_step tl tl' tl'').
+  + exact H1.
+  + apply (tl_run_small_step tl' tl'' H2).
+Qed.
+
+Lemma tl_run_step_run
+      {A: Type}
+      (tl tl' tl'': TL A)
+  : TL_run tl tl'
+    -> TL_step tl' tl''
+    -> TL_run tl tl''.
+Proof.
+  intros H1 H2.
+  induction H1.
+  ++ constructor.
+     exact H2.
+  ++ apply (tl_step_run_trans from to tl'' Hstep H2).
+  ++ apply IHTL_run in H2.
+     apply (tl_run_big_step from tl tl'' Hstep H2).
+Qed.
+
+Lemma tl_run_trans
+      {A: Type}
+      (tl tl' tl'': TL A)
+  : TL_run tl tl'
+    -> TL_run tl' tl''
+    -> TL_run tl tl''.
+Proof.
+  intros H1 H2.
+  induction H1.
+  + exact H2.
+  + apply (tl_run_big_step from to tl'' Hstep H2).
+  + apply IHTL_run in H2.
+    apply (tl_run_big_step from tl tl'' Hstep H2).
+Qed.
+
+Lemma next_derives_big
+      {A: Type}
+      (tl tl': TL A)
+      (Hderive: TL_run tl tl')
+  : TL_run (next tl) tl'.
+Proof.
+  assert (TL_run (next tl) tl)
+    as Hbefore
+      by (repeat constructor).
+  apply (tl_run_trans (next tl) tl tl' Hbefore Hderive).
+Qed.
+
+Lemma switch_derives_after_big
+      {A: Type}
+      (tl1 tl2 tl3: TL A)
+      (prop: Instant A)
+      (Hderive: TL_run tl2 tl3)
+  : TL_run (switch tl1 prop tl2) tl3.
+Proof.
+  assert (TL_run (switch tl1 prop tl2) tl2)
+    as Hrun'
+      by (repeat constructor).
+  apply (tl_run_trans (switch tl1 prop tl2) tl2 tl3 Hrun' Hderive).
+Qed.
+
+Lemma switch_derives_before_big
+      {A: Type}
+      (tl1 tl2 tl3: TL A)
+      (prop: Instant A)
+      (Hderive: TL_run tl1 tl2)
+  : TL_run (switch tl1 prop tl3) (switch tl2 prop tl3).
+Proof.
+  induction Hderive.
+  + apply tl_run_refl.
+  + apply tl_run_small_step.
+    constructor.
+    exact Hstep.
+  + apply (tl_run_trans (switch from prop tl3) (switch tl prop tl3)).
+    ++ repeat constructor.
+       exact Hstep.
+    ++ exact IHHderive.
+Qed.
+
+Lemma TL_run_is_runTL
+  : forall {I: Type -> Type}
+           {A: Type}
+           (p: Program I A)
+           (tl: TL (ISet I))
+           (int: Interp I),
+    TL_run tl (deriveTL int p tl).
+Proof.
+  induction p.
+  + intros tl int.
+    cbn.
+    apply tl_run_refl.
+  + intros tl int.
+    cbn.
+    constructor.
+    apply TL_step_is_tl_step.
+  + intros tl int.
+    cbn.
+    apply (tl_run_trans tl
+                        (snd (runTL int p tl))
+                        (snd
+                           (runTL (snd (fst (runTL int p tl))) (f (fst (fst (runTL int p tl))))
+                                  (snd (runTL int p tl))))).
+    ++ apply IHp.
+    ++ apply H.
+Qed.
+
+Inductive TL_derive
+          {A: Type}
+  : TL A -> TL A -> Prop :=
+| tl_derives_tl
+    (x: TL A)
+  : TL_derive x x
+| true_derives_true
+  : TL_derive true true
+| false_derives_false
+  : TL_derive false false
+| globally_derives_globally
+    (prop: Instant A)
+  : TL_derive (globally prop) (globally prop)
+| globally_derives_fail
+    (prop: Instant A)
+  : TL_derive (globally prop) false
+| eventually_derives_eventually
+    (prop: Instant A)
+  : TL_derive (eventually prop) (eventually prop)
+| eventually_derives_fail
+    (prop: Instant A)
+  : TL_derive (eventually prop) true
+| next_derives_unwrap
+    (tl tl': TL A)
+    (Hderive: TL_derive tl tl')
+  : TL_derive (next tl) tl'
+| switch_derives_before
+    (before after tl: TL A)
+    (prop: Instant A)
+    (Hderive: TL_derive before tl)
+  : TL_derive (switch before prop after) (switch tl prop after)
+| switch_derives_after
+    (before after tl: TL A)
+    (prop: Instant A)
+    (Hderive: TL_derive after tl)
+  : TL_derive (switch before prop after) tl
+| switch_derives_fail
+    (before after: TL A)
+    (prop: Instant A)
+  : TL_derive (switch before prop after) false.
+
+Arguments tl_derives_tl [_].
+Arguments true_derives_true [_].
+Arguments false_derives_false [_].
+Arguments globally_derives_globally [_].
+Arguments globally_derives_fail [_].
+Arguments eventually_derives_eventually [_].
+Arguments eventually_derives_fail [_].
+Arguments next_derives_unwrap [_].
+Arguments switch_derives_before [_].
+Arguments switch_derives_after [_].
+Arguments switch_derives_fail [_].
+
+Lemma tl_step_is_tl_derive
+      {A: Type}
+  : forall (tl tl': TL A),
+    TL_step  tl tl' -> TL_derive tl tl'.
+Proof.
+  induction tl; intros; inversion H; subst.
+  + constructor.
+  + constructor.
+  + constructor.
+  + constructor.
+  + constructor.
+  + constructor.
+  + constructor; constructor.
+  + constructor.
+    apply IHtl1.
+    exact Hderive.
+  + constructor; constructor.
+  + apply switch_derives_fail.
+Qed.
+
+Lemma tl_run_implies_tl_derive
+      {A: Type}
+  : forall (tl tl': TL A),
+    TL_derive tl tl' -> TL_run  tl tl'.
+Proof.
+  induction tl.
+  + intros tl' Hderive.
+    inversion Hderive; subst; constructor.
+  + intros tl' Hderive.
+    inversion Hderive; subst; constructor.
+  + intros tl' Hderive.
+    inversion Hderive; subst; repeat constructor.
+  + intros tl' Hderive.
+    inversion Hderive; subst; repeat constructor.
+  + intros tl' Hderive.
+    inversion Hderive; subst.
+    ++ apply tl_run_refl.
+    ++ assert (TL_run (next tl) tl)
+        as Hstep
+          by (repeat constructor).
+       apply (tl_run_trans (next tl) tl tl' Hstep).
+       apply IHtl.
+       apply Hderive0.
+  + intros tl' Hderive.
+    inversion Hderive; subst.
+    ++ apply tl_run_refl.
+    ++ apply (switch_derives_before_big tl1 tl tl2).
+       apply IHtl1.
+       exact Hderive0.
+    ++ apply (switch_derives_after_big tl1 tl2 tl').
+       apply IHtl2.
+       exact Hderive0.
+    ++ repeat constructor.
+Qed.
+
+Lemma switch_derives_before_helper
+      {A: Type}
+      (tl1 tl2 tl3: TL A)
+      (prop: Instant A)
+      (Hderive: TL_derive tl1 tl2)
+  : TL_derive (switch tl1 prop tl3) (switch tl2 prop tl3).
+Proof.
+  induction Hderive.
+  + constructor.
+  + constructor.
+  + constructor.
+  + constructor.
+  + repeat constructor.
+  + constructor.
+  + repeat constructor.
+  + apply switch_derives_before.
+    constructor.
+    exact Hderive.
+  + apply switch_derives_before.
+    apply switch_derives_before.
+    exact Hderive.
+  + apply switch_derives_before.
+    apply switch_derives_after.
+    exact Hderive.
+  + apply switch_derives_before.
+    apply switch_derives_fail.
+Qed.
+
+Lemma tl_derive_trans'
+      {A: Type}
+  : forall (tl tl': TL A),
+    TL_derive tl tl' -> (forall (tl'': TL A), TL_derive tl' tl'' -> TL_derive tl tl'').
+Proof.
+  intros tl tl' H1; induction H1; intros tl'' H2; try exact H2.
+  + inversion_clear H2;
+      constructor.
+  + inversion_clear H2;
+      constructor.
+  + constructor.
+    apply (IHTL_derive tl'' H2).
+  + inversion_clear H2.
+    ++ apply switch_derives_before_helper.
+       exact H1.
+    ++ apply switch_derives_before_helper.
+       apply (IHTL_derive tl0 Hderive).
+    ++ apply switch_derives_after.
+       exact Hderive.
+    ++ apply switch_derives_fail.
+  + apply switch_derives_after.
+    apply IHTL_derive in H2.
+    exact H2.
+  + inversion_clear H2.
+    ++ apply switch_derives_fail.
+    ++ apply switch_derives_fail.
+Qed.
+
+Lemma tl_derive_trans
+      {A: Type}
+  : forall (tl tl' tl'': TL A),
+    TL_derive tl tl' -> TL_derive tl' tl'' -> TL_derive tl tl''.
+Proof.
+  intros tl tl' tl'' H1 H2.
+  apply (tl_derive_trans' tl tl' H1 tl'' H2).
+Qed.
+
+Lemma tl_derive_implies_tl_run
+      {A: Type}
+  : forall (tl tl': TL A),
+    TL_run tl tl' -> TL_derive  tl tl'.
+Proof.
+  intros.
+  induction H.
+  + constructor.
+  + apply tl_step_is_tl_derive in Hstep.
+    exact Hstep.
+  + apply tl_step_is_tl_derive in Hstep.
+    apply (tl_derive_trans from tl to Hstep IHTL_run).
+Qed.
+
+Theorem derive_is_run_and_run_is_derive
         {A: Type}
         (tl tl': TL A)
-        (Hderive: TL_run tl tl')
-    : TL_run (next tl) tl'.
-  Proof.
-    assert (TL_run (next tl) tl)
-      as Hbefore
-        by (repeat constructor).
-    apply (tl_run_trans (next tl) tl tl' Hbefore Hderive).
-    Qed.
+  : TL_run tl tl' <-> TL_derive tl tl'.
+Proof.
+  split.
+  + apply tl_derive_implies_tl_run.
+  + apply tl_run_implies_tl_derive.
+Qed.
 
-  Lemma switch_derives_after_big
-        {A: Type}
-        (tl1 tl2 tl3: TL A)
-        (prop: Instant A)
-        (Hderive: TL_run tl2 tl3)
-    : TL_run (switch tl1 prop tl2) tl3.
-  Proof.
-    assert (TL_run (switch tl1 prop tl2) tl2)
-      as Hrun'
-        by (repeat constructor).
-    apply (tl_run_trans (switch tl1 prop tl2) tl2 tl3 Hrun' Hderive).
-  Qed.
+Corollary TL_derive_is_runTL
+  : forall {I: Type -> Type}
+           {A: Type}
+           (p: Program I A)
+           (tl: TL (ISet I))
+           (int: Interp I),
+    TL_derive tl (deriveTL int p tl).
+Proof.
+  intros I A p tl int.
+  apply tl_derive_implies_tl_run.
+  apply TL_run_is_runTL.
+Qed.
 
-  Lemma switch_derives_before_big
-        {A: Type}
-        (tl1 tl2 tl3: TL A)
-        (prop: Instant A)
-        (Hderive: TL_run tl1 tl2)
-    : TL_run (switch tl1 prop tl3) (switch tl2 prop tl3).
-  Proof.
-    induction Hderive.
-    + apply tl_run_refl.
-    + apply tl_run_small_step.
-      constructor.
-      exact Hstep.
-    + apply (tl_run_trans (switch from prop tl3) (switch tl prop tl3)).
-      ++ repeat constructor.
-         exact Hstep.
-      ++ exact IHHderive.
-  Qed.
-
-  Lemma TL_run_is_runTL
-    : forall {A: Type}
-             (p: Program I A)
-             (tl: TL ISet)
-             (int: Interp I),
-      TL_run tl (deriveTL int p tl).
-  Proof.
-    induction p.
-    + intros tl int.
-      cbn.
-      apply (tl_run_trans tl
-                          (snd (runTL int p tl))
-                          (snd
-                             (runTL (snd (fst (runTL int p tl))) (f (fst (fst (runTL int p tl))))
-                                    (snd (runTL int p tl))))).
-      ++ apply IHp.
-      ++ apply H.
-    + intros tl int.
-      cbn.
-      constructor.
-      apply TL_step_is_tl_step.
-    + intros tl int.
-      cbn.
-      apply tl_run_refl.
-  Qed.
-
-  Inductive TL_derive
-            {A: Type}
-    : TL A -> TL A -> Prop :=
-  | tl_derives_tl
-      (x: TL A)
-    : TL_derive x x
-  | true_derives_true
-    : TL_derive true true
-  | false_derives_false
-    : TL_derive false false
-  | globally_derives_globally
-      (prop: Instant A)
-    : TL_derive (globally prop) (globally prop)
-  | globally_derives_fail
-      (prop: Instant A)
-    : TL_derive (globally prop) false
-  | eventually_derives_eventually
-      (prop: Instant A)
-    : TL_derive (eventually prop) (eventually prop)
-  | eventually_derives_fail
-      (prop: Instant A)
-    : TL_derive (eventually prop) true
-  | next_derives_unwrap
-      (tl tl': TL A)
-      (Hderive: TL_derive tl tl')
-    : TL_derive (next tl) tl'
-  | switch_derives_before
-      (before after tl: TL A)
-      (prop: Instant A)
-      (Hderive: TL_derive before tl)
-    : TL_derive (switch before prop after) (switch tl prop after)
-  | switch_derives_after
-      (before after tl: TL A)
-      (prop: Instant A)
-      (Hderive: TL_derive after tl)
-    : TL_derive (switch before prop after) tl
-  | switch_derives_fail
-      (before after: TL A)
-      (prop: Instant A)
-    : TL_derive (switch before prop after) false.
-
-  Lemma tl_step_is_tl_derive
-        {A: Type}
-    : forall (tl tl': TL A),
-      TL_step  tl tl' -> TL_derive tl tl'.
-  Proof.
-    induction tl; intros; inversion H; subst.
-    + constructor.
-    + constructor.
-    + constructor.
-    + constructor.
-    + constructor.
-    + constructor.
-    + constructor; constructor.
-    + constructor.
-      apply IHtl1.
-      exact Hderive.
-    + constructor; constructor.
-    + apply switch_derives_fail.
-  Qed.
-
-  Lemma tl_run_implies_tl_derive
-        {A: Type}
-    : forall (tl tl': TL A),
-      TL_derive tl tl' -> TL_run  tl tl'.
-  Proof.
-    induction tl.
-    + intros tl' Hderive.
-      inversion Hderive; subst; constructor.
-    + intros tl' Hderive.
-      inversion Hderive; subst; constructor.
-    + intros tl' Hderive.
-      inversion Hderive; subst; repeat constructor.
-    + intros tl' Hderive.
-      inversion Hderive; subst; repeat constructor.
-    + intros tl' Hderive.
-      inversion Hderive; subst.
-      ++ apply tl_run_refl.
-      ++ assert (TL_run (next tl) tl)
-          as Hstep
-            by (repeat constructor).
-         apply (tl_run_trans (next tl) tl tl' Hstep).
-         apply IHtl.
-         apply Hderive0.
-    + intros tl' Hderive.
-      inversion Hderive; subst.
-      ++ apply tl_run_refl.
-      ++ apply (switch_derives_before_big tl1 tl tl2).
-         apply IHtl1.
-         exact Hderive0.
-      ++ apply (switch_derives_after_big tl1 tl2 tl').
-         apply IHtl2.
-         exact Hderive0.
-      ++ repeat constructor.
-  Qed.
-
-  Lemma switch_derives_before_helper
-        {A: Type}
-        (tl1 tl2 tl3: TL A)
-        (prop: Instant A)
-        (Hderive: TL_derive tl1 tl2)
-    : TL_derive (switch tl1 prop tl3) (switch tl2 prop tl3).
-  Proof.
-    induction Hderive.
-    + constructor.
-    + constructor.
-    + constructor.
-    + constructor.
-    + repeat constructor.
-    + constructor.
-    + repeat constructor.
-    + apply switch_derives_before.
-      constructor.
-      exact Hderive.
-    + apply switch_derives_before.
-      apply switch_derives_before.
-      exact Hderive.
-    + apply switch_derives_before.
-      apply switch_derives_after.
-      exact Hderive.
-    + apply switch_derives_before.
-      apply switch_derives_fail.
-  Qed.
-
-  Lemma tl_derive_trans'
-        {A: Type}
-    : forall (tl tl': TL A),
-      TL_derive tl tl' -> (forall (tl'': TL A), TL_derive tl' tl'' -> TL_derive tl tl'').
-  Proof.
-    intros tl tl' H1; induction H1; intros tl'' H2; try exact H2.
-    + inversion_clear H2;
-        constructor.
-    + inversion_clear H2;
-        constructor.
-    + constructor.
-      apply (IHTL_derive tl'' H2).
-    + inversion_clear H2.
-      ++ apply switch_derives_before_helper.
-         exact H1.
-      ++ apply switch_derives_before_helper.
-         apply (IHTL_derive tl0 Hderive).
-      ++ apply switch_derives_after.
-         exact Hderive.
-      ++ apply switch_derives_fail.
-    + apply switch_derives_after.
-      apply IHTL_derive in H2.
-      exact H2.
-    + inversion_clear H2.
-      ++ apply switch_derives_fail.
-      ++ apply switch_derives_fail.
-  Qed.
-
-  Lemma tl_derive_trans
-        {A: Type}
-    : forall (tl tl' tl'': TL A),
-      TL_derive tl tl' -> TL_derive tl' tl'' -> TL_derive tl tl''.
-  Proof.
-    intros tl tl' tl'' H1 H2.
-    apply (tl_derive_trans' tl tl' H1 tl'' H2).
-  Qed.
-
-  Lemma tl_derive_implies_tl_run
-        {A: Type}
-    : forall (tl tl': TL A),
-      TL_run tl tl' -> TL_derive  tl tl'.
-  Proof.
-    intros.
-    induction H.
-    + constructor.
-    + apply tl_step_is_tl_derive in Hstep.
-      exact Hstep.
-    + apply tl_step_is_tl_derive in Hstep.
-      apply (tl_derive_trans from tl to Hstep IHTL_run).
-  Qed.
-
-  Theorem derive_is_run_and_run_is_derive
-          {A: Type}
-          (tl tl': TL A)
-    : TL_run tl tl' <-> TL_derive tl tl'.
-  Proof.
-    split.
-    + apply tl_derive_implies_tl_run.
-    + apply tl_run_implies_tl_derive.
-  Qed.
-
-  Corollary TL_derive_is_runTL
-    : forall {A: Type}
-             (p: Program I A)
-             (tl: TL ISet)
-             (int: Interp I),
-      TL_derive tl (deriveTL int p tl).
-  Proof.
-    intros A p tl int.
-    apply tl_derive_implies_tl_run.
-    apply TL_run_is_runTL.
-  Qed.
-
-  Lemma tl_run_switch_before
-        {A: Type}
+Lemma tl_run_switch_before
+      {A: Type}
   : forall (tl tl' tl2: TL A)
            (prop: Instant A),
-      TL_run tl tl'
-      -> TL_run (switch tl prop tl2) (switch tl' prop tl2).
-  Proof.
-    intros tl tl' tl2 prop Hrun.
-    apply tl_run_implies_tl_derive.
-    apply tl_derive_implies_tl_run in Hrun.
-    apply switch_derives_before.
-    exact Hrun.
-  Qed.
+    TL_run tl tl'
+    -> TL_run (switch tl prop tl2) (switch tl' prop tl2).
+Proof.
+  intros tl tl' tl2 prop Hrun.
+  apply tl_run_implies_tl_derive.
+  apply tl_derive_implies_tl_run in Hrun.
+  apply switch_derives_before.
+  exact Hrun.
+Qed.
 
-  Lemma run_tl_run_program_same
-        {A: Type}
-    : forall (p: Program I A)
-             (tl: TL (ISet))
-             (int: Interp I),
-      fst (runTL int p tl) = runProgram p int.
-  Proof.
-    induction p; intros tl int; cbn.
-    + rewrite H; rewrite IHp; reflexivity.
-    + apply injective_projections; reflexivity.
-    + reflexivity.
-  Qed.
-End RUN_TL.
-
-Section TL_CONTRACT.
-  Variable (I: Type -> Type).
-
-  Record TLContract :=
+Record TLContract
+       (I: Type -> Type)
+  :=
     { tl_requirements
       : TL (ISet I)
     ; tl_promises {A: Type}
@@ -673,55 +756,315 @@ Section TL_CONTRACT.
       : typeret i -> Prop
     }.
 
-  Definition contract_step
-             {A: Type}
-             (i: I A)
-             (c: TLContract)
-    : TLContract :=
-    {| tl_requirements := tl_step (instruction _ i) (tl_requirements c)
-     ; tl_promises := fun _ i => tl_promises c i
-     |}.
+Arguments tl_requirements [_].
+Arguments tl_promises [_] (_) [_] (_ _).
 
-  Definition contract_derive
-             {A: Type}
-             (p: Program I A)
-             (int: Interp I)
-             (c: TLContract)
-    : TLContract :=
-    {| tl_requirements := deriveTL _ int p (tl_requirements c)
-     ; tl_promises := fun _ i => tl_promises c i
-     |}.
+Definition contract_step
+           {I: Type -> Type}
+           {A: Type}
+           (i: I A)
+           (c: TLContract I)
+  : TLContract I :=
+  {| tl_requirements := tl_step (instruction i) (tl_requirements c)
+   ; tl_promises := fun _ i => tl_promises c i
+  |}.
 
-  CoInductive TLEnforcer
-              (int: Interp I)
-    : TLContract -> Prop :=
-  | enforced (c: TLContract)
-             (Hprom: forall {A: Type}
-                            (i: I A),
-                 instruction_satisfies _ (instruction _ i) (tl_requirements c)
-                 -> (tl_promises c i) (evalInstruction i int))
-             (Henf:  forall {A: Type}
-                            (i: I A),
-                 instruction_satisfies _ (instruction _ i) (tl_requirements c)
-                 -> TLEnforcer (execInstruction i int) (contract_step i c))
-    : TLEnforcer int c.
+Definition contract_derive
+           {I: Type -> Type}
+           {A: Type}
+           (p: Program I A)
+           (int: Interp I)
+           (c: TLContract I)
+  : TLContract I :=
+  {| tl_requirements := deriveTL int p (tl_requirements c)
+   ; tl_promises := fun _ i => tl_promises c i
+  |}.
 
-  Inductive tl_contractfull_program
-            (c: TLContract)
-    : forall {A: Type}, Program I A -> Type :=
-  | tl_contractfull_instr {A: Type}
-                          (i: I A)
-                          (Hreq: instruction_satisfies _ (instruction _ i) (tl_requirements c))
-    : tl_contractfull_program c (instr i)
-  | tl_contractfull_ret {A: Type}
-                        (a: A)
-    : tl_contractfull_program c (ret a)
-  | tl_contractfull_inv {A B: Type}
-                        (p: Program I A)
-                        (f: A -> Program I B)
-                        (Hcp: tl_contractfull_program c p)
-                        (Hnext: forall (int: Interp I)
-                                       (Henf: TLEnforcer int (contract_derive p int c)),
-                            tl_contractfull_program (contract_derive p int c) (f (evalProgram p int)))
-    : tl_contractfull_program c (bind p f).
-End TL_CONTRACT.
+Lemma contract_derives_ret_eq
+      {I: Type -> Type}
+      {A: Type}
+      (a: A)
+      (int: Interp I)
+      (c: TLContract I)
+  : contract_derive (ret a) int c = c.
+Proof.
+  induction c.
+  split.
+Qed.
+
+Lemma contract_derives_contract_step
+      {I: Type -> Type}
+      {A: Type}
+      (i: I A)
+      (int: Interp I)
+      (c: TLContract I)
+  : contract_derive (instr i) int c = contract_step i c.
+Proof.
+  unfold contract_derive, contract_step.
+  reflexivity.
+Qed.
+
+Lemma contract_derives_bind_ret
+      {I: Type -> Type}
+      {A B: Type}
+      (a: A)
+      (f: A -> Program I B)
+      (int: Interp I)
+      (c: TLContract I)
+  : contract_derive (bind (ret a) f) int c = contract_derive (f a) int c.
+Proof.
+  reflexivity.
+Qed.
+
+CoInductive TLEnforcer
+            {I: Type -> Type}
+            (int: Interp I)
+  : TLContract I -> Prop :=
+| enforced (c: TLContract I)
+           (Hprom: forall {A: Type}
+                          (i: I A),
+               instruction_satisfies (instruction i) (tl_requirements c)
+               -> (tl_promises c i) (evalInstruction int i))
+           (Henf:  forall {A: Type}
+                          (i: I A),
+               instruction_satisfies (instruction i) (tl_requirements c)
+               -> TLEnforcer (execInstruction int i) (contract_step i c))
+  : TLEnforcer int c.
+
+Lemma enforcer_enforces_promises
+      {I: Type -> Type}
+      {A: Type}
+      (i: I A)
+      (int: Interp I)
+      (c: TLContract I)
+      (Henf: TLEnforcer int c)
+      (Hreq: instruction_satisfies (instruction i) (tl_requirements c))
+  : tl_promises c i (evalInstruction int i).
+Proof.
+  destruct Henf.
+  apply Hprom.
+  exact Hreq.
+Qed.
+
+Inductive tl_contractfull_program
+          {I: Type -> Type}
+          (c: TLContract I)
+  : forall {A: Type}, Program I A -> Prop :=
+| tl_contractfull_instr {A: Type}
+                        (i: I A)
+                        (Hreq: instruction_satisfies (instruction i) (tl_requirements c))
+  : tl_contractfull_program c (instr i)
+| tl_contractfull_ret {A: Type}
+                      (a: A)
+  : tl_contractfull_program c (ret a)
+| tl_contractfull_inv {A B: Type}
+                      (p: Program I A)
+                      (f: A -> Program I B)
+                      (Hcp: tl_contractfull_program c p)
+                      (Hnext: forall (int: Interp I)
+                                     (Henf: TLEnforcer int c),
+                          tl_contractfull_program (contract_derive p int c) (f (evalProgram int p)))
+  : tl_contractfull_program c (bind p f).
+
+Lemma contractfull_program_bind_ret
+      {I: Type -> Type}
+      {A B: Type}
+      (a: A)
+      (f: A -> Program I B)
+      (c: TLContract I)
+  : tl_contractfull_program c (f a) -> tl_contractfull_program c (bind (ret a) f).
+Proof.
+  intros Hp.
+  constructor.
+  + constructor.
+  + intros int Henf.
+    cbn.
+    rewrite contract_derives_ret_eq.
+    exact Hp.
+Qed.
+
+Conjecture contractfull_program_bind_ret'
+  : forall {I: Type -> Type}
+           {A B: Type}
+           (a: A)
+           (f: A -> Program I B)
+           (c: TLContract I),
+    tl_contractfull_program c (bind (ret a) f) -> tl_contractfull_program c (f a).
+
+Lemma enforcer_instruction_contractfull_enforcer
+      {I: Type -> Type}
+      {A: Type}
+      (i: I A)
+      (int: Interp I)
+      (c: TLContract I)
+      (H: TLEnforcer int c)
+      (Hp: tl_contractfull_program c (instr i))
+  : TLEnforcer (execTL int (instr i) (tl_requirements c)) (contract_derive (instr i) int c).
+Proof.
+  cbn.
+  constructor.
+  + intros B i' Hinst.
+    destruct H as [c Hprom Henf].
+    inversion Hp.
+    apply Henf in Hreq.
+    apply inj_pair2 in H1.
+    subst.
+    inversion Hreq.
+    rewrite contract_derives_contract_step.
+    apply Hprom0.
+    exact Hinst.
+  + intros B i' Hinst.
+    destruct H as [c Hprom Henf].
+    inversion Hp.
+    apply Henf in Hreq.
+    apply inj_pair2 in H1.
+    subst.
+    inversion Hreq.
+    rewrite contract_derives_contract_step.
+    apply Henf0.
+    exact Hinst.
+Qed.
+
+Lemma enforcer_ret_contractfull_enforcer
+      {I: Type -> Type}
+      {A: Type}
+      (a: A)
+      (int: Interp I)
+      (c: TLContract I)
+      (H: TLEnforcer int c)
+  : TLEnforcer (execTL int (ret a) (tl_requirements c)) (contract_derive (ret a) int c).
+Proof.
+  rewrite (contract_derives_ret_eq a int c).
+  unfold execTL.
+  cbn.
+  exact H.
+Qed.
+
+Lemma contract_derive_assoc
+      {I: Type -> Type}
+      {A B C: Type}
+      (p: Program I A)
+      (f: A -> Program I B)
+      (f': B -> Program I C)
+      (int: Interp I)
+      (c: TLContract I)
+  : contract_derive (bind (bind p f) f') int c
+    = contract_derive (bind p (fun x => bind (f x) f')) int c.
+Proof.
+  reflexivity.
+Qed.
+
+Lemma exec_program_assoc'
+      (I: Type -> Type)
+      {A: Type}
+      (p: Program I A)
+  : forall {B C: Type}
+           (f: A -> Program I B)
+           (f': B -> Program I C)
+           (int: Interp I),
+    execProgram int (bind (bind p f) f')
+    = execProgram int (bind p (fun x => (bind (f x) f'))).
+Proof.
+  intros B C f f' int.
+  reflexivity.
+Qed.
+
+Lemma exec_tl_assoc
+      {I: Type -> Type}
+      {A: Type}
+      (p: Program I A)
+  : forall {B: Type}
+           (f: A -> Program I B)
+           (int: Interp I)
+           (c: TLContract I),
+    execTL int (bind p f) (tl_requirements c)
+    = execTL (execTL int p (tl_requirements c))
+             (f (evalProgram int p)) (tl_requirements (contract_derive p int c)).
+Proof.
+  intros B f int c.
+  repeat rewrite exec_tl_exec_program_same.
+  reflexivity.
+Qed.
+
+Lemma eval_program_assoc
+      {I: Type -> Type}
+      {A: Type}
+      (p: Program I A)
+  : forall {B: Type}
+           (f: A -> Program I B)
+           (int: Interp I)
+           (c: TLContract I),
+    evalProgram int (bind p f)
+    = evalProgram (execTL int p (tl_requirements c))
+                  (f (evalProgram int p)).
+Proof.
+  intros B f int c.
+  rewrite exec_tl_exec_program_same.
+  reflexivity.
+Qed.
+
+Lemma contract_derive_bind
+      {I: Type -> Type}
+      {A: Type}
+      (p: Program I A)
+  : forall {B: Type}
+           (f: A -> Program I B)
+           (int: Interp I)
+           (c: TLContract I),
+    contract_derive (f (evalProgram int p)) (execTL int p (tl_requirements c)) (contract_derive p int c) = contract_derive (bind p f) int c.
+Proof.
+  induction p.
+  + reflexivity.
+  + reflexivity.
+  + intros C f' int' c'.
+    rewrite contract_derive_assoc.
+    rewrite <- (IHp C) .
+    rewrite <- H.
+    rewrite <- eval_program_assoc.
+    rewrite <- exec_tl_assoc.
+    rewrite <- (IHp A) .
+    reflexivity.
+Qed.
+
+Lemma execTL_bind
+      {I: Type -> Type}
+      {A B: Type}
+      (p: Program I A)
+  : forall (f: A -> Program I B)
+           (int: Interp I)
+           (c: TLContract I),
+    execTL (execTL int p (tl_requirements c)) (f (evalProgram int p)) (tl_requirements (contract_derive p int c)) = execTL int (bind p f) (tl_requirements c).
+Proof.
+  intros f int c.
+  repeat rewrite exec_tl_exec_program_same.
+  reflexivity.
+Qed.
+
+Lemma enforcer_contractfull_enforcer
+      {I: Type -> Type}
+      {A: Type}
+      (p: Program I A)
+  : forall (c: TLContract I)
+           (int: Interp I)
+           (H: TLEnforcer int c)
+           (Hp: tl_contractfull_program c p),
+    TLEnforcer (execTL int p (tl_requirements c)) (contract_derive p int c).
+Proof.
+  induction p.
+  + intros c int He Hp;
+      apply (enforcer_ret_contractfull_enforcer a int c He).
+  + intros c int He Hp;
+      apply (enforcer_instruction_contractfull_enforcer i int c He Hp).
+  + intros c int He Hp.
+    inversion Hp;
+      apply inj_pair2 in H3;
+      repeat apply inj_pair2 in H4;
+      subst.
+    apply (IHp c int He) in Hcp.
+    rewrite <- execTL_bind.
+    rewrite <- contract_derive_bind.
+    apply H.
+    ++ exact Hcp.
+    ++ apply Hnext.
+       exact He.
+Qed.
